theories/concurrent/ws_deque.v
@@ -16,40 +16,40 @@ Record ws_deque `{!heapGS Σ} := {
 
   ws_deque_inv : val → namespace → iProp Σ ;
   ws_deque_model : val → list val → iProp Σ ;
-  ws_deque_own : val → iProp Σ ;
+  ws_deque_owner : val → iProp Σ ;
 
   ws_deque_inv_persistent t ι :
     Persistent (ws_deque_inv t ι) ;
   ws_deque_model_timeless t vs :
     Timeless (ws_deque_model t vs) ;
-  ws_deque_own_timeless t :
-    Timeless (ws_deque_own t) ;
+  ws_deque_owner_timeless t :
+    Timeless (ws_deque_owner t) ;
 
-  ws_deque_own_exclusive t :
-    ws_deque_own t -∗
-    ws_deque_own t -∗
+  ws_deque_owner_exclusive t :
+    ws_deque_owner t -∗
+    ws_deque_owner t -∗
     False ;
 
   ws_deque_make_spec ι :
     {{{ True }}}
       ws_deque_make #()
-    {{{ t, RET t; ws_deque_inv t ι ∗ ws_deque_model t [] ∗ ws_deque_own t }}} ;
+    {{{ t, RET t; ws_deque_inv t ι ∗ ws_deque_model t [] ∗ ws_deque_owner t }}} ;
 
   ws_deque_push_spec t ι v :
     <<<
-      ws_deque_inv t ι ∗ ws_deque_own t |
+      ws_deque_inv t ι ∗ ws_deque_owner t |
       ∀∀ vs, ws_deque_model t vs
     >>>
       ws_deque_push t v
       @ ↑ ι
     <<<
       ws_deque_model t (vs ++ [v]) |
-      RET #(); ws_deque_own t
+      RET #(); ws_deque_owner t
     >>> ;
 
   ws_deque_pop_spec t ι :
     <<<
-      ws_deque_inv t ι ∗ ws_deque_own t |
+      ws_deque_inv t ι ∗ ws_deque_owner t |
       ∀∀ vs, ws_deque_model t vs
     >>>
       ws_deque_pop t
@@ -57,7 +57,7 @@ Record ws_deque `{!heapGS Σ} := {
     <<< ∃∃ o,
       (⌜vs = [] ∧ o = NONEV⌝ ∗ ws_deque_model t []) ∨
       (∃ vs' v, ⌜vs = vs' ++ [v] ∧ o = SOMEV v⌝ ∗ ws_deque_model t vs') |
-      RET o; ws_deque_own t
+      RET o; ws_deque_owner t
     >>> ;
 
   ws_deque_steal_spec t ι :
@@ -77,4 +77,4 @@ Record ws_deque `{!heapGS Σ} := {
 #[global] Arguments Build_ws_deque {_ _ _ _ _ _ _ _ _ _ _ _} _ _ _ _ _ : assert.
 #[global] Existing Instance ws_deque_inv_persistent.
 #[global] Existing Instance ws_deque_model_timeless.
-#[global] Existing Instance ws_deque_own_timeless.
+#[global] Existing Instance ws_deque_owner_timeless.
